equivalence subloop

src/Distributions/DiscreteLaplace/Equivalence.dfy
@@ -11,6 +11,7 @@ module DiscreteLaplace.Equivalence {
   import Uniform
   import Coin
   import Model
+  import Loops
 
   /************
    Definitions
@@ -36,14 +37,25 @@ module DiscreteLaplace.Equivalence {
           SampleTailRecursive(scale, b, y)(s)
   }
 
-  ghost function SampleTailRecursiveHelper(a: bool := true, v: int := 0): Monad.Hurd<int> {
-    assume {:axiom} false; // assume termination
-    (s: Rand.Bitstream) =>
-      if !a then
-        Monad.Result(v, s)
-      else
-        var (a, s) :- BernoulliExpNeg.Model.Sample(Rationals.Int(1))(s);
-        SampleTailRecursiveHelper(a, if a then v + 1 else v)(s)
+  ghost function SampleTailRecursiveHelper(): Monad.Hurd<int> 
+    requires Loops.WhileCutTerminates(Model.SampleHelperLoopCondition, Model.SampleHelperLoopBody, (true, 0), s)   
+  {
+    var f := (x: (bool, int)) => x.1;
+    Monad.Map(SampleTailRecursiveHelperLoop(), f)
+  }
+
+  ghost function SampleTailRecursiveHelperLoop(x: (bool, int) := (true, 0)): Monad.Hurd<(bool, int)> 
+    requires Loops.WhileCutTerminates(Model.SampleHelperLoopCondition, Model.SampleHelperLoopBody, x, s) 
+  {
+    var fuel := Loops.LeastFuel(Model.SampleHelperLoopCondition, Model.SampleHelperLoopBody, x, s);
+    SampleTailRecursiveHelperLoopCut(x, fuel)
+  }
+
+  ghost function SampleTailRecursiveHelperLoopCut(x: (bool, int) := (true, 0), fuel): Monad.Hurd<(bool, int)> {
+    if fuel == 0 || !x.0 then 
+      Monad.Return(x)
+    else
+      Monad.Bind(Model.SamplerHelperLoopBody(x), (x': (bool, int)) => SampleTailRecursiveHelperLoop(x', fuel - 1))
   }
 
   /*******
@@ -53,4 +65,67 @@ module DiscreteLaplace.Equivalence {
   lemma {:axiom} SampleTailRecursiveEquivalence(scale: Rationals.Rational, s: Rand.Bitstream)
     requires scale.numer >= 1
     ensures SampleTailRecursive(scale)(s) == Model.Sample(scale)(s)
+
+  lemma SampleTailRecursiveHelperEquivalence(s: Rand.Bitstream)
+    ensures SampleTailRecursiveHelper()(s) == Model.SampleHelper()(s)
+  {
+    var f := (x: (bool, int)) => x.1;
+    var (x, s') :- SampleTailRecursiveHelperLoop((true, 0))(s);
+    var (x', s'') :- Model.SampleHelperLoop((true, 0))(s);
+    calc {
+      SampleTailRecursiveHelper()(s);
+      Monad.Map(SampleTailRecursiveHelperLoop(), f)(s);
+      Monad.Bind(SampleTailRecursiveHelperLoop(), (x: bool, int) => Monad.Return(f(x)))(s);
+      Monad.Return(f(x'))(s');
+      { assert x == x' && s' == s'' by { SampleTailRecursiveHelperCutEquivalence((ture, 0), s) }; }
+      Monad.Return(f(x''))(s'');
+      Monad.Bind(Model.SampleHelperLoop(), (x: bool, int) => Monad.Return(f(x)));
+      Monad.Map(Model.SampleHelperLoop(), f)(s);
+      Model.SampleHelper()(s);
+    }
+  }
+
+  lemma SampleTailRecursiveHelperCutEquivalence(x: (bool, int), s: Rand.Bitstream)
+    requires Loops.WhileCutTerminates(Model.SampleHelperLoopCondition, Model.SampleHelperLoopBody, x, s) 
+    ensures SampleTailRecursiveHelperLoop(x)(s) == Model.SampleHelperLoop(x)(s)
+  {
+    var fuel := Loops.LeastFuel(Model.SampleHelperLoopCondition, Model.SampleHelperLoopBody, x, s);
+    calc {
+      SampleTailRecursiveHelperLoop(x)(s);
+      SampleTailRecursiveHelperLoopCut(x, fuel)(s);
+      { SampleTailRecursiveHelperCutEquivalence(x, s, fuel); }
+      Loops.WhileCut(SampleHelperLoopCondition, SampleHelperLoopBody, x, fuel)(s);
+      Loops.While(SampleHelperLoopCondition, SampleHelperLoopBody)(x)(s);
+      Model.SampleHelperLoop(x)(s);
+    }
+  }
+
+  lemma SampleTailRecursiveHelperCutEquivalence(x: (bool, int), s: Rand.Bitstream, fuel: nat)
+    ensures SampleTailRecursiveHelperLoopCut(x, fuel)(s) == Loops.WhileCut(SampleHelperLoopCondition, SampleHelperLoopBody, x, fuel)(s)
+  {
+    if !x.0 {
+      calc {
+        SampleTailRecursiveHelperLoopCut(x, fuel)(s)
+        Monad.Return(x)(s);
+        Loops.WhileCut(SampleHelperLoopCondition, SampleHelperLoopBody, x, fuel)(s);
+      }
+    } else if fuel == 0 {
+      calc {
+        SampleTailRecursiveHelperLoopCut(x, fuel)(s)
+        Monad.Return(x)(s);
+        Loops.WhileCut(SampleHelperLoopCondition, SampleHelperLoopBody, x, fuel)(s)
+      }
+    } else {
+      var (x', s') :- Model.SamplerHelperLoopBody(x)(s);
+      calc {
+        SampleTailRecursiveHelperLoopCut(x, fuel)(s);
+        Monad.Bind(Model.SamplerHelperLoopBody(x), (x': (bool, int)) => SampleTailRecursiveHelperLoopCut(x', fuel - 1))(s);
+        SampleTailRecursiveHelperLoopCut(x', fuel - 1)(s');
+        { SampleTailRecursiveHelperEquivalence(x', s', fuel - 1); }
+        Loops.WhileCut(SampleHelperLoopCondition, SampleHelperLoopBody, x', fuel - 1)(s');
+        Monad.Bind(Model.SampleHelperLoopBody(x), (x': (bool, int) => Loops.WhileCut(SampleHelperLoopCondition, SampleHelperLoopBody, x', fuel - 1)))(s);
+        Monad.Bind(Model.SampleHelperLoopBody(x), (x': (bool, int) => Loops.WhileCut(SampleHelperLoopCondition, SampleHelperLoopBody, x', fuel - 1)))(s);
+        Loops.WhileCut(SampleHelperLoopCondition, SampleHelperLoopBody, x, fuel)(s)
+    }
+  }
 }
